TseitinProofs.fst
@@ -19,6 +19,22 @@ let rec append_valid_cnf_formulas (f1 : list (list int)) (f2 : list (list int))
       else append_valid_cnf_formulas (tl f1) f2
 
 
+let rec append_variables_in_interval (f1 : list (list int)) (f2 : list (list int))
+                                     (n:nat) (start_interval:nat) (end_interval:nat)
+    : Lemma (requires n <= start_interval /\ start_interval <= end_interval /\
+                      valid_cnf_formula f1 /\ valid_cnf_formula f2 /\
+                      variables_in_interval f1 n start_interval end_interval /\
+                      variables_in_interval f2 n start_interval end_interval)
+            (ensures valid_cnf_formula (f1 @ f2) /\ variables_in_interval (f1 @ f2) n start_interval end_interval)
+    = append_valid_cnf_formulas f1 f2;
+      if f1 = [] then ()
+      else 
+      (
+          append_valid_cnf_formulas (L.tl f1) f2;
+          append_variables_in_interval (tl f1) f2 n start_interval end_interval
+      )
+
+
 let prove_same_value_not (f1:formula_t) (rf1 : list (list int)) (v1:int) (n:nat)
                          (start_interval:nat) (end_interval:nat) (rf : list (list int)) (v:int)
     : Lemma (requires n <= start_interval /\ start_interval <= v /\
@@ -30,9 +46,29 @@ let prove_same_value_not (f1:formula_t) (rf1 : list (list int)) (v1:int) (n:nat)
                      tseitin_same_value (Not f1) rf v n start_interval end_interval)
     = append_valid_cnf_formulas rf1 (not_clauses v1 v);
 
+      variables_in_interval_monotone rf1 n start_interval v end_interval;
+      assert (variables_in_interval rf1 n start_interval end_interval);
 
+      let nc = not_clauses v1 v in
+      assert (variables_in_interval_literal (L.index (L.index nc 0) 0) n start_interval end_interval);
+      assert (variables_in_interval_literal (L.index (L.index nc 0) 1) n start_interval end_interval);
+      assert (variables_in_interval_literal (L.index (L.index nc 1) 0) n start_interval end_interval);
+      assert (variables_in_interval_literal (L.index (L.index nc 1) 1) n start_interval end_interval);
+      // assert (L.index nc 0 = [L.index (L.index nc 0) 0; L.index (L.index nc 0) 1]);
+      assert (L.index nc 0 = [L.index (L.index nc 0) 0; L.index (L.index nc 0) 1] &&
+              variables_in_interval_literal (L.index (L.index nc 0) 0) n start_interval end_interval &&
+              variables_in_interval_literal (L.index (L.index nc 0) 1) n start_interval end_interval ==>
+              variables_in_interval_clause (L.index nc 0) n start_interval end_interval);
+      // assert (variables_in_interval_clause (L.index nc 0) n start_interval end_interval);
+      assert (L.index nc 1 = [L.index (L.index nc 1) 0; L.index (L.index nc 1) 1]);
+      assert (variables_in_interval_clause (L.index nc 1) n start_interval end_interval);
+      assert (variables_in_interval nc n start_interval end_interval);
+
+      assert (variables_in_interval (not_clauses v1 v) n start_interval end_interval);
+
+      append_variables_in_interval rf1 (not_clauses v1 v) n start_interval end_interval;
       assert (variables_in_interval rf n start_interval end_interval);
-      // assert (valid (Not f1) rf v n start_interval end_interval);
+      assert (valid (Not f1) rf v n start_interval end_interval);
 
       let aux (tau : list bool) 
           : Lemma (requires L.length tau >= end_interval /\
@@ -184,24 +220,108 @@ let prove_same_value_not (f1:formula_t) (rf1 : list (list int)) (v1:int) (n:nat)
   
 
 // let prove_can_extend_not (f1:formula_t) (rf1 : list (list int)) (v1:int) (n:nat)
-//                          (start_interval:nat) (end_interval:nat) (rf : list (list int)) (v:int)
+//                          (start_interval:nat) (v:int) (end_interval:nat) (rf : list (list int))
 //     : Lemma (requires n <= start_interval /\ start_interval <= v /\ v < end_interval /\
 //                       valid f1 rf1 v1 n start_interval v /\
 //                       tseitin_can_extend f1 rf1 v1 n start_interval v /\
-//                       rf = L.append rf1 (not_clauses v1 v) /\ end_interval = v + 1)
+//                       rf = rf1 @ (not_clauses v1 v) /\
+//                       end_interval = v + 1)
 //             (ensures valid (Not f1) rf v n start_interval end_interval /\
 //                      tseitin_can_extend (Not f1) rf v n start_interval end_interval)
-//     = assert (n <= v);
-//       assert (valid (Not f1) rf v n start_interval end_interval);
-//       let aux (tau : list bool) : Lemma (requires L.length tau = n)
-//                                         (ensures can_extend tau (Not f1) rf v n start_interval end_interval)
+//     = assert (valid (Not f1) rf v n start_interval end_interval);
+//       let aux (tau : list bool) 
+//           : Lemma (requires L.length tau = n)
+//                   (ensures can_extend tau (Not f1) rf v n start_interval end_interval)
 //           = assert (can_extend tau f1 rf1 v1 n start_interval v);
 //             assert (valid_literal (pos_var_to_lit v1));
-//             // let ghost tau1 : list bool = exists (tau1 : list bool) . L.length tau1 = v in
-//             // negate_literal v1 tau1
-//             // let (|tau1, _|) = exists (tau1 : list bool) . L.length tau1 = v in
-//             // negate_literal v1 tau1     
-//             let tau1 = exists_elim (exists (tau1 : list bool) . L.length tau1 = v) in
-//             negate_literal v1 tau1
+            
+//             let conditions (tau1 : list bool) =
+//                 // tau <= tau1 /\
+//                 L.length tau1 = v /\
+//                 truth_value_cnf_formula rf1 tau1 /\
+//                 truth_value f1 tau = truth_value_literal (pos_var_to_lit v1) tau1
+//             in
+//             let extract_from_exists : (tau1 : list bool {conditions tau1}) -> prop = fun (tau1 : list bool) -> conditions tau1 in
+//             let tau1 : list bool = FStar.IndefiniteDescription.indefinite_description_ghost (list bool) extract_from_exists in
+
+//             negate_literal v1 tau1;
+
+//             let tau' = combine1 tau tau1 n start_interval v (truth_value (Not f1) tau) in
+//             // assert (tau <= tau');
+//             assert (L.length tau' = end_interval);
+//             transfer_truth_value rf1 tau1 tau' n start_interval v;
+
+//             transfer_truth_value_lit (pos_var_to_lit v1) tau1 tau' n start_interval v;
+//             assert (truth_value_literal (pos_var_to_lit v1) tau' = truth_value f1 tau);
+//             transfer_truth_value_lit (neg_var_to_lit v1) tau1 tau' n start_interval v;
+//             assert (truth_value_literal (neg_var_to_lit v1) tau1 = not (truth_value_literal (pos_var_to_lit v1) tau1));
+
+//             lemma_not_clauses v1 v tau';
+//             assert (truth_value_cnf_formula rf tau')
 //       in
 //       forall_intro (move_requires aux) 
+
+
+// let prove_can_extend_or (f1:formula_t) (rf1 : list (list int)) (v1:int) 
+//                         (f2:formula_t) (rf2 : list (list int)) (v2:int) 
+//                         (n:nat) (start_interval:nat) (mid:nat) (v:int) (end_interval:nat)
+//                         (rf :list (list int))
+//     : Lemma (requires n <= start_interval /\ start_interval <= mid /\ mid <= v /\
+//                       valid f1 rf1 v1 n start_interval mid /\
+//                       tseitin_can_extend f1 rf1 v1 n start_interval mid /\
+//                       valid f2 rf2 v2 n mid v /\
+//                       tseitin_can_extend f2 rf2 v2 n mid v /\
+//                       rf = rf1 @ rf2 @ (or_clauses v1 v2 v) /\
+//                       end_interval = v + 1)
+//             (ensures valid (Or f1 f2) rf v n start_interval end_interval /\
+//                      tseitin_can_extend (Or f1 f2) rf v n start_interval end_interval)
+//     = assert (valid (Or f1 f2) rf v n start_interval end_interval);
+//       let aux (tau : list bool)
+//           : Lemma (requires L.length tau = n)
+//                   (ensures can_extend tau (Or f1 f2) rf v n start_interval end_interval)
+//           = let conditions (tau1 : list bool) =
+//                 // tau <= tau1 /\
+//                 L.length tau1 = mid /\
+//                 truth_value_cnf_formula rf1 tau1 /\
+//                 truth_value f1 tau = truth_value_literal (pos_var_to_lit v1) tau1
+//             in
+//             let extract_from_exists : (tau1 : list bool {conditions tau1}) -> prop = fun (tau1 : list bool) -> conditions tau1 in
+//             let tau1 : list bool = FStar.IndefiniteDescription.indefinite_description_ghost (list bool) extract_from_exists in
+
+//             let conditions (tau2 : list bool) =
+//                 // tau <= tau2 /\
+//                 L.length tau2 = v /\
+//                 truth_value_cnf_formula rf2 tau2 /\
+//                 truth_value f2 tau = truth_value_literal (pos_var_to_lit v2) tau2
+//             in
+//             let extract_from_exists : (tau2 : list bool {conditions tau2}) -> prop = fun (tau2 : list bool) -> conditions tau2 in
+//             let tau2 : list bool = FStar.IndefiniteDescription.indefinite_description_ghost (list bool) extract_from_exists in
+
+//             let tau' = combine tau tau1 tau2 n start_interval mid v (truth_value (Or f1 f2) tau) in
+
+//             assert (interval_of_list tau' 0 n = interval_of_list tau 0 n);
+//             assert (interval_of_list tau' start_interval mid = interval_of_list tau1 start_interval mid);
+//             assert (interval_of_list tau' mid v = interval_of_list tau2 mid v);
+//             assert (L.index tau' v = truth_value (Or f1 f2) tau);
+
+//             assert (truth_value_literal (pos_var_to_lit v) tau' = truth_value (Or f1 f2) tau);
+//             assert (truth_value_literal (neg_var_to_lit v) tau' = not (truth_value (Or f1 f2) tau));
+
+//             transfer_truth_value rf1 tau1 tau' n start_interval mid;
+//             transfer_truth_value rf2 tau2 tau' n mid v;
+
+//             transfer_truth_value_lit (pos_var_to_lit v1) tau1 tau' n start_interval mid;
+//             transfer_truth_value_lit (neg_var_to_lit v1) tau1 tau' n start_interval mid;
+//             assert (truth_value_literal (pos_var_to_lit v1) tau' = truth_value f1 tau);
+//             assert (truth_value_literal (neg_var_to_lit v1) tau' = not (truth_value f1 tau));
+
+//             transfer_truth_value_lit (pos_var_to_lit v2) tau2 tau' n mid v;
+//             transfer_truth_value_lit (neg_var_to_lit v2) tau2 tau' n mid v;
+//             assert (truth_value_literal (pos_var_to_lit v2) tau' = truth_value f2 tau);
+//             assert (truth_value_literal (neg_var_to_lit v2) tau' = not (truth_value f2 tau));
+
+//             assert (truth_value (Or f1 f2) tau = truth_value f1 tau || truth_value f2 tau);
+//             lemma_or_clauses v1 v2 v tau';
+//             assert (can_extend tau (Or f1 f2) rf v n start_interval end_interval)
+//       in
+//       forall_intro (move_requires aux)
